<?xml version="1.0"?>


<!DOCTYPE rdf:RDF [
    <!ENTITY dcterms "http://purl.org/dc/terms/" >
    <!ENTITY owl "http://www.w3.org/2002/07/owl#" >
    <!ENTITY dc "http://purl.org/dc/elements/1.1/" >
    <!ENTITY xsd "http://www.w3.org/2001/XMLSchema#" >
    <!ENTITY rdfs "http://www.w3.org/2000/01/rdf-schema#" >
    <!ENTITY rdf "http://www.w3.org/1999/02/22-rdf-syntax-ns#" >
    <!ENTITY vs "http://www.w3.org/2003/06/sw-vocab-status/ns#" >
]>


<rdf:RDF xmlns="http://entropy-project.eu/behavioral#"
     xml:base="http://entropy-project.eu/behavioral"
     xmlns:dc="http://purl.org/dc/elements/1.1/"
     xmlns:rdfs="http://www.w3.org/2000/01/rdf-schema#"
     xmlns:owl="http://www.w3.org/2002/07/owl#"
     xmlns:xsd="http://www.w3.org/2001/XMLSchema#"
     xmlns:rdf="http://www.w3.org/1999/02/22-rdf-syntax-ns#"
     xmlns:vs="http://www.w3.org/2003/06/sw-vocab-status/ns#"
     xmlns:dcterms="http://purl.org/dc/terms/">
    <owl:Ontology rdf:about="http://entropy-project.eu/behavioural">
        <rdfs:label>ENTROPY Behavioural Intervention Ontology</rdfs:label>
        <dcterms:created rdf:datatype="&xsd;dateTime">2016-08-16</dcterms:created>
        <dcterms:licence rdf:datatype="&xsd;string">This work is licensed under a Creative Commons Attribution License (version 3.0) &lt;http://creativecommons.org/licenses/by/3.0/&gt;</dcterms:licence>
        <rdfs:comment>This ontology is designed to represent behavioural interventions in terms of recommendation and persuasive messages.</rdfs:comment>
        <dc:creator>Anna Fensel (University of Innsbruck, STI Innsbruck)</dc:creator>
        <dc:contributor>Angeliki Bousiou (INTELEN Inc.)</dc:contributor>
        <dc:creator>Umutcan Simsek (University of Innsbruck, STI Innsbruck)</dc:creator>
        <dcterms:publisher rdf:resource="http://sti2.at"/>
        <owl:versionIRI rdf:resource="http://entropy-project.eu/behavioural/1.0.0"/>
    </owl:Ontology>
    


    <!-- 
    ///////////////////////////////////////////////////////////////////////////////////////
    //
    // Annotation properties
    //
    ///////////////////////////////////////////////////////////////////////////////////////
     -->

    


    <!-- http://purl.org/dc/elements/1.1/contributor -->

    <owl:AnnotationProperty rdf:about="&dc;contributor"/>
    


    <!-- http://purl.org/dc/elements/1.1/creator -->

    <owl:AnnotationProperty rdf:about="&dc;creator"/>
    


    <!-- http://purl.org/dc/elements/1.1/description -->

    <owl:AnnotationProperty rdf:about="&dc;description"/>
    


    <!-- http://www.w3.org/2003/06/sw-vocab-status/ns#term_status -->

    <owl:AnnotationProperty rdf:about="&vs;term_status">
        <rdfs:comment>&apos;unstable&apos;
    The meaning, deployment practices, documentation (or important associated software/services) associated with this term are liable to change arbitrarily at some point in the future. They may not, but stability is not guaranteed. Use with caution.
&apos;testing&apos;
    The meaning, deployment practices, documentation and general understanding of this term are approaching some stability, but changes are still possible due to implementation experience or other unanticipated factors.
&apos;stable&apos;
    The term is relatively stable, and its documentation and meaning are not expected to change substantially.
&apos;archaic&apos;
    This term is marked as old-fashioned; although used, it is not considered typical of current best practice and alternative expressions may be preferable. </rdfs:comment>
        <rdfs:seeAlso rdf:resource="https://www.w3.org/2003/06/sw-vocab-status/note"/>
    </owl:AnnotationProperty>
    


    <!-- 
    ///////////////////////////////////////////////////////////////////////////////////////
    //
    // Object Properties
    //
    ///////////////////////////////////////////////////////////////////////////////////////
     -->

    


    <!-- http://entropy-project.eu/behavioural#activity -->

    <owl:ObjectProperty rdf:about="http://entropy-project.eu/behavioural#activity">
        <rdfs:label>activity</rdfs:label>
        <rdfs:comment>The property that relates a Task to an Activity.</rdfs:comment>
        <vs:term_status>testing</vs:term_status>
        <rdfs:range rdf:resource="http://entropy-project.eu/behavioural#Activity"/>
        <rdfs:domain rdf:resource="http://entropy-project.eu/behavioural#Task"/>
    </owl:ObjectProperty>
    


    <!-- http://entropy-project.eu/behavioural#currentSituation -->

    <owl:ObjectProperty rdf:about="http://entropy-project.eu/behavioural#currentSituation">
        <rdfs:label>current situation</rdfs:label>
        <vs:term_status>unstable</vs:term_status>
        <rdfs:comment>The property that relates a Person to a Situation. (see Situation)</rdfs:comment>
        <rdfs:range rdf:resource="http://entropy-project.eu/behavioural#Situation"/>
        <rdfs:domain rdf:resource="http://xmlns.com/foaf/0.1/Person"/>
    </owl:ObjectProperty>
    


    <!-- http://entropy-project.eu/behavioural#difficulty -->

    <owl:ObjectProperty rdf:about="http://entropy-project.eu/behavioural#difficulty">
        <rdfs:label>difficulty level</rdfs:label>
        <vs:term_status>unstable</vs:term_status>
        <rdfs:comment>A Task can have a Difficulty level</rdfs:comment>
        <rdfs:range rdf:resource="http://entropy-project.eu/behavioural#Difficulty"/>
        <rdfs:domain rdf:resource="http://entropy-project.eu/behavioural#Task"/>
    </owl:ObjectProperty>
    


    <!-- http://entropy-project.eu/behavioural#educationalLevel -->

    <owl:ObjectProperty rdf:about="http://entropy-project.eu/behavioural#educationalLevel">
        <rdfs:label>educational level</rdfs:label>
        <rdfs:comment>The property that indicates a person&apos;s educational level.</rdfs:comment>
        <vs:term_status>unstable</vs:term_status>
        <rdfs:range rdf:resource="http://entropy-project.eu/behavioural#EducationalLevel"/>
        <rdfs:domain rdf:resource="http://xmlns.com/foaf/0.1/Person"/>
    </owl:ObjectProperty>
    


    <!-- http://entropy-project.eu/behavioural#feedbackTarget -->

    <owl:ObjectProperty rdf:about="http://entropy-project.eu/behavioural#feedbackTarget">
        <rdfs:label>feedback target</rdfs:label>
        <vs:term_status>unstable</vs:term_status>
        <rdfs:comment>The property that relates a Feedback to a Recommendation</rdfs:comment>
        <rdfs:domain rdf:resource="http://entropy-project.eu/behavioural#Feedback"/>
        <rdfs:range rdf:resource="http://entropy-project.eu/behavioural#Intervention"/>
    </owl:ObjectProperty>
    


    <!-- http://entropy-project.eu/behavioural#givesFeedback -->

    <owl:ObjectProperty rdf:about="http://entropy-project.eu/behavioural#givesFeedback">
        <rdfs:label>gives feedback</rdfs:label>
        <rdfs:comment>The property that indicates the Person who gives a certain Feedback.</rdfs:comment>
        <vs:term_status>unstable</vs:term_status>
        <rdfs:range rdf:resource="http://entropy-project.eu/behavioural#Feedback"/>
        <rdfs:domain rdf:resource="http://xmlns.com/foaf/0.1/Person"/>
    </owl:ObjectProperty>
    


    <!-- http://entropy-project.eu/behavioural#hasDevice -->

    <owl:ObjectProperty rdf:about="http://entropy-project.eu/behavioural#hasDevice">
        <rdfs:label>has device</rdfs:label>
        <rdfs:comment>An Agent can have a Device.</rdfs:comment>
        <vs:term_status>unstable</vs:term_status>
        <rdfs:range rdf:resource="http://cenitmio.es/ontologies/Device.owl#Device"/>
        <rdfs:domain rdf:resource="http://xmlns.com/foaf/0.1/Agent"/>
    </owl:ObjectProperty>
    


    <!-- http://entropy-project.eu/behavioural#hasPersona -->

    <owl:ObjectProperty rdf:about="http://entropy-project.eu/behavioural#hasPersona">
        <rdfs:label>has persona</rdfs:label>
        <rdfs:comment>A Person can have Persona(s)</rdfs:comment>
        <vs:term_status>unstable</vs:term_status>
        <rdfs:range rdf:resource="http://entropy-project.eu/behavioural#Persona"/>
        <rdfs:domain rdf:resource="http://xmlns.com/foaf/0.1/Person"/>
    </owl:ObjectProperty>
    


    <!-- http://entropy-project.eu/behavioural#nextTask -->

    <owl:ObjectProperty rdf:about="http://entropy-project.eu/behavioural#nextTask">
        <rdfs:label>next task</rdfs:label>
        <rdfs:comment>The property that indicates that next Task in a Task sequence.</rdfs:comment>
        <vs:term_status>testing</vs:term_status>
        <rdfs:range rdf:resource="http://entropy-project.eu/behavioural#Task"/>
        <rdfs:domain rdf:resource="http://entropy-project.eu/behavioural#Task"/>
        <owl:inverseOf rdf:resource="http://entropy-project.eu/behavioural#previousTask"/>
    </owl:ObjectProperty>
    


    <!-- http://entropy-project.eu/behavioural#previousTask -->

    <owl:ObjectProperty rdf:about="http://entropy-project.eu/behavioural#previousTask">
        <rdfs:label>previous task</rdfs:label>
        <rdfs:comment>see nextTask</rdfs:comment>
        <vs:term_status>testing</vs:term_status>
        <rdfs:range rdf:resource="http://entropy-project.eu/behavioural#Task"/>
        <rdfs:domain rdf:resource="http://entropy-project.eu/behavioural#Task"/>
    </owl:ObjectProperty>
    


    <!-- http://entropy-project.eu/behavioural#targetUser -->

    <owl:ObjectProperty rdf:about="http://entropy-project.eu/behavioural#targetUser">
        <rdfs:label>target user</rdfs:label>
        <rdfs:comment>An intervention has a target user which is an Agent.</rdfs:comment>
        <vs:term_status>testing</vs:term_status>
        <rdfs:domain rdf:resource="http://entropy-project.eu/behavioural#Intervention"/>
        <rdfs:range rdf:resource="http://xmlns.com/foaf/0.1/Agent"/>
    </owl:ObjectProperty>
    


    <!-- http://purl.org/ontology/wi/core#preference -->

    <owl:ObjectProperty rdf:about="http://purl.org/ontology/wi/core#preference">
        <rdfs:label>has preference</rdfs:label>
        <rdfs:comment>A link between an agent and a weighted interest</rdfs:comment>
        <vs:term_status>unstable</vs:term_status>
        <rdfs:isDefinedBy rdf:resource="http://purl.org/ontology/wi/core#"/>
        <rdfs:range rdf:resource="http://purl.org/ontology/wi/core#WeightedInterest"/>
        <rdfs:domain rdf:resource="http://xmlns.com/foaf/0.1/Agent"/>
    </owl:ObjectProperty>
    


    <!-- http://xmlns.com/foaf/0.1/account -->

    <owl:ObjectProperty rdf:about="http://xmlns.com/foaf/0.1/account">
        <rdfs:label>account</rdfs:label>
        <rdfs:comment>The property that relates an Agent to an Online Account</rdfs:comment>
        <vs:term_status>stable</vs:term_status>
        <rdfs:isDefinedBy rdf:resource="http://xmlns.com/foaf/0.1/"/>
        <rdfs:domain rdf:resource="http://xmlns.com/foaf/0.1/Agent"/>
        <rdfs:range rdf:resource="http://xmlns.com/foaf/0.1/OnlineAccount"/>
    </owl:ObjectProperty>
    


    <!-- http://xmlns.com/foaf/0.1/member -->

    <owl:ObjectProperty rdf:about="http://xmlns.com/foaf/0.1/member">
        <rdfs:label>member</rdfs:label>
        <rdfs:comment>The property that indicates that an Agent is a member of a Group</rdfs:comment>
        <vs:term_status>stable</vs:term_status>
        <rdfs:isDefinedBy rdf:resource="http://xmlns.com/foaf/0.1/"/>
        <rdfs:domain rdf:resource="http://xmlns.com/foaf/0.1/Agent"/>
        <rdfs:range rdf:resource="http://xmlns.com/foaf/0.1/Group"/>
    </owl:ObjectProperty>
    


    <!-- 
    ///////////////////////////////////////////////////////////////////////////////////////
    //
    // Data properties
    //
    ///////////////////////////////////////////////////////////////////////////////////////
     -->

    


    <!-- http://entropy-project.eu/behavioural#completionMessage -->

    <owl:DatatypeProperty rdf:about="http://entropy-project.eu/behavioural#completionMessage">
        <rdfs:label>completion message</rdfs:label>
        <rdfs:comment>This property indicates the textual message to be shown after the completion of a Task.</rdfs:comment>
        <vs:term_status>testing</vs:term_status>
        <rdfs:domain rdf:resource="http://entropy-project.eu/behavioural#Task"/>
        <rdfs:range rdf:resource="&xsd;string"/>
    </owl:DatatypeProperty>
    


    <!-- http://entropy-project.eu/behavioural#weeklyHours -->

    <owl:DatatypeProperty rdf:about="http://entropy-project.eu/behavioural#weeklyHours">
        <rdfs:label>weekly hours</rdfs:label>
        <vs:term_status>stable</vs:term_status>
        <rdfs:comment>Weekly hours of an employee. Value of this property may be used for behavioural analytics</rdfs:comment>
        <rdfs:domain rdf:resource="http://entropy-project.eu/behavioural#Employee"/>
        <rdfs:range rdf:resource="&xsd;integer"/>
    </owl:DatatypeProperty>
    


    <!-- http://xmlns.com/foaf/0.1/age -->

    <owl:DatatypeProperty rdf:about="http://xmlns.com/foaf/0.1/age">
        <rdfs:label>age</rdfs:label>
        <rdfs:comment>Age of an Agent</rdfs:comment>
        <vs:term_status>stable</vs:term_status>
        <rdfs:isDefinedBy rdf:resource="http://xmlns.com/foaf/0.1/"/>
        <rdfs:domain rdf:resource="http://xmlns.com/foaf/0.1/Agent"/>
    </owl:DatatypeProperty>
    


    <!-- 
    ///////////////////////////////////////////////////////////////////////////////////////
    //
    // Classes
    //
    ///////////////////////////////////////////////////////////////////////////////////////
     -->

    


    <!-- http://cenitmio.es/ontologies/Device.owl#Device -->

    <owl:Class rdf:about="http://cenitmio.es/ontologies/Device.owl#Device">
        <rdfs:label>Device</rdfs:label>
        <vs:term_status>unstable</vs:term_status>
        <rdfs:comment>A Device</rdfs:comment>
        <rdfs:isDefinedBy rdf:resource="http://cenitmio.es/ontologies/Device.owl"/>
    </owl:Class>
    


    <!-- http://cenitmio.es/ontologies/Device.owl#MobileDevice -->

    <owl:Class rdf:about="http://cenitmio.es/ontologies/Device.owl#MobileDevice">
        <rdfs:label>Mobile Device</rdfs:label>
        <rdfs:subClassOf rdf:resource="http://cenitmio.es/ontologies/Device.owl#Device"/>
        <vs:term_status>unstable</vs:term_status>
        <rdfs:comment>A portable device</rdfs:comment>
        <rdfs:isDefinedBy rdf:resource="http://cenitmio.es/ontologies/Device.owl"/>
    </owl:Class>
    


    <!-- http://cenitmio.es/ontologies/Device.owl#MobilePhone -->

    <owl:Class rdf:about="http://cenitmio.es/ontologies/Device.owl#MobilePhone">
        <rdfs:label>Mobile Phone</rdfs:label>
        <rdfs:subClassOf rdf:resource="http://cenitmio.es/ontologies/Device.owl#MobileDevice"/>
        <vs:term_status>unstable</vs:term_status>
        <rdfs:comment>A mobile phone. This class represents mobile phone of a person and its properties that may be used to identify a person or its certain context elements.</rdfs:comment>
        <rdfs:isDefinedBy rdf:resource="http://cenitmio.es/ontologies/Device.owl"/>
    </owl:Class>
    


    <!-- http://entropy-project.eu/behavioural#Activity -->

    <owl:Class rdf:about="http://entropy-project.eu/behavioural#Activity">
        <rdfs:label>Activity</rdfs:label>
        <rdfs:comment>An activity can be part of task. Every instance of an activity or its subclasses might have different properties depending on activities nature. 

e.g. Walk activity can have a distance property.</rdfs:comment>
        <vs:term_status>unstable</vs:term_status>
    </owl:Class>
    


    <!-- http://entropy-project.eu/behavioural#Bike -->

    <owl:Class rdf:about="http://entropy-project.eu/behavioural#Bike">
        <rdfs:label>Bike</rdfs:label>
        <rdfs:subClassOf rdf:resource="http://entropy-project.eu/behavioural#OutdoorActivity"/>
        <vs:term_status>unstable</vs:term_status>
        <rdfs:comment>Biking activity</rdfs:comment>
    </owl:Class>
    


    <!-- http://entropy-project.eu/behavioural#CloseWindow -->

    <owl:Class rdf:about="http://entropy-project.eu/behavioural#CloseWindow">
        <rdfs:subClassOf rdf:resource="http://entropy-project.eu/behavioural#IndoorActivity"/>
    </owl:Class>
    


    <!-- http://entropy-project.eu/behavioural#Difficulty -->

    <owl:Class rdf:about="http://entropy-project.eu/behavioural#Difficulty">
        <rdfs:label>Difficulty</rdfs:label>
        <rdfs:comment>This class represents difficulty levels. A typical usage of a difficulty instance is a Task.</rdfs:comment>
        <vs:term_status>unstable</vs:term_status>
    </owl:Class>
    


    <!-- http://entropy-project.eu/behavioural#EducationalLevel -->

    <owl:Class rdf:about="http://entropy-project.eu/behavioural#EducationalLevel">
        <rdfs:label>Educational Level</rdfs:label>
        <vs:term_status>unstable</vs:term_status>
        <rdfs:comment>Educational level may be used for behavioural analysis and recommendations.</rdfs:comment>
    </owl:Class>
    


    <!-- http://entropy-project.eu/behavioural#Employee -->

    <owl:Class rdf:about="http://entropy-project.eu/behavioural#Employee">
        <rdfs:label>Employee</rdfs:label>
        <rdfs:subClassOf rdf:resource="http://xmlns.com/foaf/0.1/Person"/>
        <rdfs:comment>A subclass of Person that represents the people who work at an institution.</rdfs:comment>
        <vs:term_status>unstable</vs:term_status>
    </owl:Class>
    


    <!-- http://entropy-project.eu/behavioural#FacebookAccount -->

    <owl:Class rdf:about="http://entropy-project.eu/behavioural#FacebookAccount">
        <rdfs:label>Facebook Account</rdfs:label>
        <rdfs:subClassOf rdf:resource="http://xmlns.com/foaf/0.1/OnlineAccount"/>
        <vs:term_status>unstable</vs:term_status>
        <rdfs:comment>A subclass of OnlineAccount. It may be used to identify a person or to retrieve some profile information for behavioural analysis.</rdfs:comment>
    </owl:Class>
    


    <!-- http://entropy-project.eu/behavioural#Feedback -->

    <owl:Class rdf:about="http://entropy-project.eu/behavioural#Feedback">
        <rdfs:label>Feedback</rdfs:label>
        <rdfs:comment>People can give positive or negative feedback to a recommendation.</rdfs:comment>
        <vs:term_status>unstable</vs:term_status>
    </owl:Class>
    


    <!-- http://entropy-project.eu/behavioural#FinalTask -->

    <owl:Class rdf:about="http://entropy-project.eu/behavioural#FinalTask">
        <rdfs:label>Final Task</rdfs:label>
        <rdfs:subClassOf rdf:resource="http://entropy-project.eu/behavioural#Task"/>
        <rdfs:subClassOf>
            <owl:Restriction>
                <owl:onProperty rdf:resource="http://entropy-project.eu/behavioural#nextTask"/>
                <owl:maxCardinality rdf:datatype="&xsd;nonNegativeInteger">0</owl:maxCardinality>
            </owl:Restriction>
        </rdfs:subClassOf>
        <rdfs:comment>The final task of a sequence.</rdfs:comment>
    </owl:Class>
    


    <!-- http://entropy-project.eu/behavioural#IndoorActivity -->

    <owl:Class rdf:about="http://entropy-project.eu/behavioural#IndoorActivity">
        <rdfs:label>Indoor Activity</rdfs:label>
        <rdfs:subClassOf rdf:resource="http://entropy-project.eu/behavioural#Activity"/>
        <vs:term_status>unstable</vs:term_status>
        <rdfs:comment>A supertype of indoor activities. These activities can be part of a task.</rdfs:comment>
    </owl:Class>
    


    <!-- http://entropy-project.eu/behavioural#Intervention -->

    <owl:Class rdf:about="http://entropy-project.eu/behavioural#Intervention">
        <rdfs:label>Intervention</rdfs:label>
        <vs:term_status>testing</vs:term_status>
        <rdfs:comment>This class represents an intervention aiming to change a certain behaviour. An intervention can be in different forms (e.g Task, Message).</rdfs:comment>
    </owl:Class>
    


    <!-- http://entropy-project.eu/behavioural#Message -->

    <owl:Class rdf:about="http://entropy-project.eu/behavioural#Message">
        <rdfs:label>Message</rdfs:label>
        <rdfs:subClassOf rdf:resource="http://entropy-project.eu/behavioural#Intervention"/>
        <vs:term_status>testing</vs:term_status>
        <rdfs:comment>The Message class represents a persuasive message targeting a person.</rdfs:comment>
    </owl:Class>
    


    <!-- http://entropy-project.eu/behavioural#NegativeFeedback -->

    <owl:Class rdf:about="http://entropy-project.eu/behavioural#NegativeFeedback">
        <rdfs:label>Negative Feedback</rdfs:label>
        <rdfs:subClassOf rdf:resource="http://entropy-project.eu/behavioural#Feedback"/>
        <owl:disjointWith rdf:resource="http://entropy-project.eu/behavioural#PositiveFeedback"/>
        <vs:term_status>unstable</vs:term_status>
    </owl:Class>
    


    <!-- http://entropy-project.eu/behavioural#OpenWindow -->

    <owl:Class rdf:about="http://entropy-project.eu/behavioural#OpenWindow">
        <rdfs:subClassOf rdf:resource="http://entropy-project.eu/behavioural#IndoorActivity"/>
    </owl:Class>
    


    <!-- http://entropy-project.eu/behavioural#OutdoorActivity -->

    <owl:Class rdf:about="http://entropy-project.eu/behavioural#OutdoorActivity">
        <rdfs:label>Outdoor Activity</rdfs:label>
        <rdfs:subClassOf rdf:resource="http://entropy-project.eu/behavioural#Activity"/>
        <rdfs:comment>A supertype of outdoor activities. These activities can be part of a task.</rdfs:comment>
        <vs:term_status>unstable</vs:term_status>
    </owl:Class>
    


    <!-- http://entropy-project.eu/behavioural#Persona -->

    <owl:Class rdf:about="http://entropy-project.eu/behavioural#Persona">
        <rdfs:label>Persona</rdfs:label>
        <rdfs:comment>This class represents a persona label, produced by behavioural analysis.</rdfs:comment>
        <vs:term_status>unstable</vs:term_status>
    </owl:Class>
    


    <!-- http://entropy-project.eu/behavioural#PositiveFeedback -->

    <owl:Class rdf:about="http://entropy-project.eu/behavioural#PositiveFeedback">
        <rdfs:label>Positive Feedback</rdfs:label>
        <rdfs:subClassOf rdf:resource="http://entropy-project.eu/behavioural#Feedback"/>
        <vs:term_status>unstable</vs:term_status>
    </owl:Class>
    


    <!-- http://entropy-project.eu/behavioural#Situation -->

    <owl:Class rdf:about="http://entropy-project.eu/behavioural#Situation">
        <rdfs:label>Situation</rdfs:label>
        <vs:term_status>unstable</vs:term_status>
        <rdfs:comment>Current sitution of a user. Situation is inferred by context reasoning based on different context elements (time, location etc.)</rdfs:comment>
    </owl:Class>
    


    <!-- http://entropy-project.eu/behavioural#Student -->

    <owl:Class rdf:about="http://entropy-project.eu/behavioural#Student">
        <rdfs:label>Student</rdfs:label>
        <rdfs:subClassOf rdf:resource="http://xmlns.com/foaf/0.1/Person"/>
        <vs:term_status>unstable</vs:term_status>
        <rdfs:comment>A student in an educational organization. The seperation between a student and an employee is important, since they have different movement patterns during a day. (e.g. students usually do not have dedicated offices, they are more felixable in terms of location)</rdfs:comment>
    </owl:Class>
    


    <!-- http://entropy-project.eu/behavioural#Task -->

    <owl:Class rdf:about="http://entropy-project.eu/behavioural#Task">
        <rdfs:label>Task</rdfs:label>
        <rdfs:subClassOf rdf:resource="http://entropy-project.eu/behavioural#Intervention"/>
        <rdfs:comment>Task is a form of recommendation. A task can be followed by another Task which forms a sequence. Every task contains an activity.</rdfs:comment>
        <vs:term_status>testing</vs:term_status>
    </owl:Class>
    


    <!-- http://entropy-project.eu/behavioural#TurnLightsOff -->

    <owl:Class rdf:about="http://entropy-project.eu/behavioural#TurnLightsOff">
        <rdfs:subClassOf rdf:resource="http://entropy-project.eu/behavioural#IndoorActivity"/>
    </owl:Class>
    


    <!-- http://entropy-project.eu/behavioural#TurnLightsOn -->

    <owl:Class rdf:about="http://entropy-project.eu/behavioural#TurnLightsOn">
        <rdfs:subClassOf rdf:resource="http://entropy-project.eu/behavioural#IndoorActivity"/>
    </owl:Class>
    


    <!-- http://entropy-project.eu/behavioural#Walk -->

    <owl:Class rdf:about="http://entropy-project.eu/behavioural#Walk">
        <rdfs:label>Walk</rdfs:label>
        <rdfs:subClassOf rdf:resource="http://entropy-project.eu/behavioural#OutdoorActivity"/>
        <vs:term_status>unstable</vs:term_status>
        <rdfs:comment>Walking activity</rdfs:comment>
    </owl:Class>
    


    <!-- http://entropy-project.eu/gamification#Quiz -->

    <owl:Class rdf:about="http://entropy-project.eu/gamification#Quiz">
        <rdfs:label>Quiz</rdfs:label>
        <rdfs:subClassOf rdf:resource="http://entropy-project.eu/behavioural#Intervention"/>
        <rdfs:comment>A gamified quiz</rdfs:comment>
        <rdfs:isDefinedBy rdf:resource="http://entropy-project.eu/gamification"/>
    </owl:Class>
    


    <!-- http://purl.org/ontology/wi/core#WeightedInterest -->

    <owl:Class rdf:about="http://purl.org/ontology/wi/core#WeightedInterest">
        <rdfs:label>Weighted Interest</rdfs:label>
        <vs:term_status>unstable</vs:term_status>
        <rdfs:comment>A weighted interest object, which also can have interest dynamics etc. This concept may be used to represent questionaire and/or survey results for behavioural analysis.</rdfs:comment>
        <rdfs:isDefinedBy rdf:resource="http://purl.org/ontology/wi/core#"/>
    </owl:Class>
    


    <!-- http://xmlns.com/foaf/0.1/Agent -->

    <owl:Class rdf:about="http://xmlns.com/foaf/0.1/Agent">
        <rdfs:label>Agent</rdfs:label>
        <rdfs:comment>The Agent class is the class of agents; things that do stuff.</rdfs:comment>
        <vs:term_status>stable</vs:term_status>
        <rdfs:isDefinedBy rdf:resource="http://xmlns.com/foaf/0.1/"/>
        <rdfs:seeAlso rdf:resource="http://xmlns.com/foaf/spec/#term_Agent"/>
    </owl:Class>
    


    <!-- http://xmlns.com/foaf/0.1/Group -->

    <owl:Class rdf:about="http://xmlns.com/foaf/0.1/Group">
        <rdfs:label>Group</rdfs:label>
        <rdfs:subClassOf rdf:resource="http://xmlns.com/foaf/0.1/Agent"/>
        <vs:term_status>stable</vs:term_status>
        <rdfs:comment>The Group class represents a collection of individual agents (and may itself play the role of a Agent, ie. something that can perform actions).

In the context of this vocabulary, Group concept represents a group of people that share some common characteristics. Group instances may be created by behavioural analysis and be used in recommendation process.</rdfs:comment>
        <rdfs:isDefinedBy rdf:resource="http://xmlns.com/foaf/0.1/"/>
    </owl:Class>
    


    <!-- http://xmlns.com/foaf/0.1/OnlineAccount -->

    <owl:Class rdf:about="http://xmlns.com/foaf/0.1/OnlineAccount">
        <rdfs:label>Online Account</rdfs:label>
        <rdfs:comment>The OnlineAccount class represents the provision of some form of online service, by some party  to some Agent.</rdfs:comment>
        <vs:term_status>stable</vs:term_status>
        <rdfs:isDefinedBy rdf:resource="http://xmlns.com/foaf/0.1/"/>
    </owl:Class>
    


    <!-- http://xmlns.com/foaf/0.1/Person -->

    <owl:Class rdf:about="http://xmlns.com/foaf/0.1/Person">
        <rdfs:label>Person</rdfs:label>
        <rdfs:subClassOf rdf:resource="http://xmlns.com/foaf/0.1/Agent"/>
        <vs:term_status>stable</vs:term_status>
        <rdfs:comment>The Person class represents people.</rdfs:comment>
        <rdfs:isDefinedBy rdf:resource="http://xmlns.com/foaf/0.1/"/>
    </owl:Class>
    


    <!-- 
    ///////////////////////////////////////////////////////////////////////////////////////
    //
    // Individuals
    //
    ///////////////////////////////////////////////////////////////////////////////////////
     -->

    


    <!-- http://cenitmio.es/ontologies/Device.owl#Easy -->

    <owl:NamedIndividual rdf:about="http://cenitmio.es/ontologies/Device.owl#Easy">
        <rdf:type rdf:resource="http://entropy-project.eu/behavioural#Difficulty"/>
    </owl:NamedIndividual>
    


    <!-- http://entropy-project.eu/behavioural#Doctor -->

    <owl:NamedIndividual rdf:about="http://entropy-project.eu/behavioural#Doctor">
        <rdf:type rdf:resource="http://entropy-project.eu/behavioural#EducationalLevel"/>
        <rdfs:label>Doctorate Degree</rdfs:label>
    </owl:NamedIndividual>
    


    <!-- http://entropy-project.eu/behavioural#Hard -->

    <owl:NamedIndividual rdf:about="http://entropy-project.eu/behavioural#Hard">
        <rdf:type rdf:resource="http://entropy-project.eu/behavioural#Difficulty"/>
    </owl:NamedIndividual>
    


    <!-- http://entropy-project.eu/behavioural#HighSchool -->

    <owl:NamedIndividual rdf:about="http://entropy-project.eu/behavioural#HighSchool">
        <rdf:type rdf:resource="http://entropy-project.eu/behavioural#EducationalLevel"/>
        <rdfs:label>High School Diploma</rdfs:label>
    </owl:NamedIndividual>
    


    <!-- http://entropy-project.eu/behavioural#Master -->

    <owl:NamedIndividual rdf:about="http://entropy-project.eu/behavioural#Master">
        <rdf:type rdf:resource="http://entropy-project.eu/behavioural#EducationalLevel"/>
        <rdfs:label>Master&apos;s Degree</rdfs:label>
    </owl:NamedIndividual>
    


    <!-- http://entropy-project.eu/behavioural#Medium -->

    <owl:NamedIndividual rdf:about="http://entropy-project.eu/behavioural#Medium">
        <rdf:type rdf:resource="http://entropy-project.eu/behavioural#Difficulty"/>
    </owl:NamedIndividual>
    


    <!-- http://entropy-project.eu/behavioural#Undergraduate -->

    <owl:NamedIndividual rdf:about="http://entropy-project.eu/behavioural#Undergraduate">
        <rdf:type rdf:resource="http://entropy-project.eu/behavioural#EducationalLevel"/>
        <rdfs:label>Undergraduate Degree</rdfs:label>
    </owl:NamedIndividual>
</rdf:RDF>



<!-- Generated by the OWL API (version 3.4.2) http://owlapi.sourceforge.net -->

